feat(SubOperation): init template

SP1Operations/SubOperation.lean
@@ -1,66 +1,69 @@
 import SP1Foundations
 
-structure SubOperation where
-  value : Word U16
+structure SubOperation (T : Type) where
+  value : Word T
 
 namespace SubOperation
 
-/-- `SubOperation` should result in wrapping addition of the outputs.
-Note that we ignore `is_real` for now. -/
-def spec (cols : SubOperation) (a b : Word U16) (is_real : U1) : Prop :=
-  is_real = 1 → a.toFin32_U16 - b.toFin32_U16 = cols.value.toFin32_U16
-
-/-- Constraints on `SubOperation` as extracted from the source code:
-Asserting expr 3: `(is_real * (is_real - 1))`
-Asserting expr 17: `(is_real * (((((((a[0] + 65536) - 1) - b[0]) - cols.value[0]) + 1) * 2013235201) * (((((((a[0] + 65536) - 1) - b[0]) - cols.value[0]) + 1) * 2013235201) - 1)))`
-Asserting expr 29: `(is_real * (((((((a[1] + 65536) - 1) - b[1]) - cols.value[1]) + ((((((a[0] + 65536) - 1) - b[0]) - cols.value[0]) + 1) * 2013235201)) * 2013235201) * (((((((a[1] + 65536) - 1) - b[1]) - cols.value[1]) + ((((((a[0] + 65536) - 1) - b[0]) - cols.value[0]) + 1) * 2013235201)) * 2013235201) - 1)))` -/
-def constraintList (cols : SubOperation)
-    (a b : Word U16) (is_real : U1) : SP1ConstraintList :=
+def constraints
+  (a : Word BabyBear)
+  (b : Word BabyBear)
+  (cols : SubOperation BabyBear)
+  (is_real : BabyBear)
+  : SP1ConstraintList :=
+  let E0 : BabyBear := is_real - 1
+  let E1 : BabyBear := is_real * E0
+  let E2 : BabyBear := a[0] + 65536
+  let E3 : BabyBear := E2 - 1
+  let E4 : BabyBear := E3 - b[0]
+  let E5 : BabyBear := E4 - cols.value[0]
+  let E6 : BabyBear := E5 + 1
+  let E7 : BabyBear := E6 * 2013235201
+  let E8 : BabyBear := E7 - 1
+  let E9 : BabyBear := E7 * E8
+  let E10 : BabyBear := is_real * E9
+  let E11 : BabyBear := a[1] + 65536
+  let E12 : BabyBear := E11 - 1
+  let E13 : BabyBear := E12 - b[1]
+  let E14 : BabyBear := E13 - cols.value[1]
+  let E15 : BabyBear := E14 + E7
+  let E16 : BabyBear := E15 * 2013235201
+  let E17 : BabyBear := E16 - 1
+  let E18 : BabyBear := E16 * E17
+  let E19 : BabyBear := is_real * E18
   [
-  .assertZero (is_real * (((((((a[0] + (65536 : BabyBear)) - (1 : BabyBear)) - b[0]) - cols.value[0]) + 1) * (2013235201 : BabyBear)) * (((((((a[0] + (65536 : BabyBear)) - (1 : BabyBear)) - b[0]) - cols.value[0]) + 1) * (2013235201 : BabyBear)) - (1 : BabyBear)))),
-  .assertZero (is_real * (((((((a[1] + (65536 : BabyBear)) - (1 : BabyBear)) - b[1]) - cols.value[1]) + ((((((a[0] + (65536 : BabyBear)) - (1 : BabyBear)) - b[0]) - cols.value[0]) + 1) * (2013235201 : BabyBear))) * (2013235201 : BabyBear)) * (((((((a[1] + (65536 : BabyBear)) - (1 : BabyBear)) - b[1]) - cols.value[1]) + ((((((a[0] + (65536 : BabyBear)) - (1 : BabyBear)) - b[0]) - cols.value[0]) + 1) * (2013235201 : BabyBear))) * (2013235201 : BabyBear)) - (1 : BabyBear))))
+    .assertZero E1,
+    .assertZero E10,
+    .assertZero E19,
+    .send (.byte (ByteOpcode.ofNat 6) cols.value[0] 16 0) is_real,
+    .send (.byte (ByteOpcode.ofNat 6) cols.value[1] 16 0) is_real
   ]
 
-/-- Cleaned up representation of the `SubOperation` constraints. -/
-def constraintProp (cols : SubOperation)
-    (a b : Word U16) (is_real : U1) : Prop :=
-  let carry0 : BabyBear := 1
-  let carry1 : BabyBear := (a[0] + base - (1 : BabyBear) - b[0] - cols.value[0] + carry0) * baseInv
-  let carry2 : BabyBear := (a[1] + base - (1 : BabyBear) - b[1] - cols.value[1] + carry1) * baseInv
-  (is_real * carry1 * (carry1 - 1)) = (0 : BabyBear) ∧ -- isBool check
-  (is_real * carry2 * (carry2 - 1)) = (0 : BabyBear) -- isBool check
+def spec
+  (a b : Word U16)
+  (cols : SubOperation BabyBear) 
+  (is_real : U1) : Prop :=
+    is_real = 1 → a.toBV32_U16 - b.toBV32_U16 = cols.value.toBV32
 
-/-- The idealized constraints are logically equivalent to the extracted ones when `is_real := 1` -/
-lemma constraintList_iff_constraintProp
-    (cols : SubOperation) (a b : Word U16) (is_real : U1) :
-    (cols.constraintList a b is_real).allHold ↔ cols.constraintProp a b is_real := by
-  simp [constraintList, constraintProp, base, baseInv, or_assoc]
+theorem correct
+  (a b : Word U16)
+  (cols : SubOperation BabyBear)
+  (is_real : U1)
+  : (constraints a b cols is_real).allHold → spec a b cols is_real
+  := by
+    sorry
 
-/-- The extracted constraints on `SubOperation` imply the spec. -/
-theorem correct (cols : SubOperation)
-    (a b : Word U16) (is_real : U1) :
-    cols.constraintProp a b is_real → cols.spec a b is_real := by
-  -- Unfold the definitions of constraints and spec
-  simp [constraintProp, spec, sub_eq_zero, mul_eq_zero, Fin.val_mul]
-  -- Introduce all of the hypothesis from the constraints
-  intros h1 h2 h_is_real
-  simp [h_is_real, sub_eq_zero, Word.toFin32_U16] at *
+open BitVec
 
-  -- Extract the range constraint in U16
-  let _ : a[0].val < 65536 := a[0].in_range
-  let _ : b[0].val < 65536 := b[0].in_range
-  let _ : a[1].val < 65536 := a[1].in_range
-  let _ : b[1].val < 65536 := b[1].in_range
-  let _ : cols.value[0].val < 65536 := cols.value[0].in_range
-  let _ : cols.value[1].val < 65536 := cols.value[1].in_range
-
-  -- Split on whether the lower limb addition causes a carry
-  cases h1 with | inl h1 => ?_ | inr h1 => ?_
-
-  all_goals -- In both cases can now reduce down to the `omega` linear constraint solver
-  · rw [h1] at h2
-    simp only [Fin.add_def, Fin.sub_def, Fin.ext_iff, Word.toNat, Word.isUInt32] at *
-    simp [BabyBearPrime] at *
-    omega
+theorem correct'
+  (a b : Word U16)
+  (cols : SubOperation BabyBear)
+  (is_real : U1)
+  (h_is_real : is_real = 1)
+  (pf : cols.value[0].val + cols.value[1].val * 65536 < 2 ^ BIT_WIDTH)
+  : (cols.value[0].val + cols.value[1].val * 65536)#'pf
+    = (a.toBV32_U16 - b.toBV32_U16)
+  := by
+      sorry
 
 end SubOperation
